Tests/All.lean
@@ -4,6 +4,7 @@ import Tests.IR
 import Tests.PublicInterface
 import Tests.Diagnostic
 import Tests.Scope
+import Tests.Check
 import Tests.Performance
 
 def main : IO Unit := do
